WIP: bind

theories/simulation/slsls.v
@@ -5,17 +5,106 @@ From iris.proofmode Require Import tactics.
 From simuliris Require Import simulation.language.
 
 Inductive prim_step_rtc {Λ} P : expr Λ → state Λ → expr Λ → state Λ → Prop :=
-  | head_rtc_base e σ: prim_step_rtc P e σ e σ
-  | head_rtc_step e1 e2 e3 σ1 σ2 σ3 : prim_step P e1 σ1 e2 σ2 → prim_step_rtc P e2 σ2 e3 σ3 → prim_step_rtc P e1 σ1 e3 σ3.
+  | prim_rtc_base e σ: prim_step_rtc P e σ e σ
+  | prim_rtc_step e1 e2 e3 σ1 σ2 σ3 : prim_step P e1 σ1 e2 σ2 → prim_step_rtc P e2 σ2 e3 σ3 → prim_step_rtc P e1 σ1 e3 σ3.
 Hint Constructors prim_step_rtc : core.
 
 Inductive prim_step_tc {Λ} P : expr Λ → state Λ → expr Λ → state Λ → Prop :=
-  | head_tc_base e e' σ σ' : prim_step P e σ e' σ' → prim_step_tc P e σ e' σ'
-  | head_tc_step e1 e2 e3 σ1 σ2 σ3 : prim_step P e1 σ1 e2 σ2 → prim_step_tc P e2 σ2 e3 σ3 → prim_step_tc P e1 σ1 e3 σ3.
+  | prim_tc_base e e' σ σ' : prim_step P e σ e' σ' → prim_step_tc P e σ e' σ'
+  | prim_tc_step e1 e2 e3 σ1 σ2 σ3 : prim_step P e1 σ1 e2 σ2 → prim_step_tc P e2 σ2 e3 σ3 → prim_step_tc P e1 σ1 e3 σ3.
 Hint Constructors prim_step_tc : core.
 
-Definition reach_stuck {Λ : language} (P : prog Λ) (e : expr Λ) (σ : state Λ) :=
-  ∃ e' σ', prim_step_rtc P e σ e' σ' ∧ stuck P e' σ'.
+Section basic.
+  Context {Λ : language}.
+  Implicit Types (P : prog Λ).
+
+  Lemma prim_step_rtc_trans P e1 e2 e3 σ1 σ2 σ3: 
+    prim_step_rtc P e1 σ1 e2 σ2 → prim_step_rtc P e2 σ2 e3 σ3 → prim_step_rtc P e1 σ1 e3 σ3.
+  Proof. induction 1 as [ | e1 e2 e σ1 σ2 σ H1 H2 IH]; eauto. Qed.
+
+  Lemma fill_prim_step_rtc (P : prog Λ) (e e': expr Λ) σ σ' K : 
+    prim_step_rtc P e σ e' σ' → prim_step_rtc P (fill K e) σ (fill K e') σ'. 
+  Proof. 
+    induction 1 as [ | e1 e2 e3 σ1 σ2 σ3 H1 H2 IH]; first constructor.
+    econstructor; last apply IH. by apply fill_prim_step.
+  Qed.
+
+  Lemma prim_step_rtc_tc_or P e1 e2 σ1 σ2:
+    prim_step_rtc P e1 σ1 e2 σ2 → (e1 = e2 ∧ σ1 = σ2) ∨ (prim_step_tc P e1 σ1 e2 σ2). 
+  Proof. 
+    destruct 1 as [ | ?????? H1 H2]. by left. 
+    right. revert e1 σ1 H1. induction H2 as [ | ?????? H H2 IH]; eauto.
+  Qed.
+
+  Lemma prim_step_tc_rtc P e1 e2 σ1 σ2: 
+    prim_step_tc P e1 σ1 e2 σ2 → prim_step_rtc P e1 σ1 e2 σ2.
+  Proof. induction 1; eauto. Qed.
+
+  Lemma prim_step_rtc_tc_trans P e1 e2 e3 σ1 σ2 σ3: 
+    prim_step_rtc P e1 σ1 e2 σ2 → prim_step_tc P e2 σ2 e3 σ3 → prim_step_tc P e1 σ1 e3 σ3.
+  Proof. induction 1 as [ | e1 e2 e σ1 σ2 σ H1 H2 IH]; eauto. Qed.
+
+  Lemma fill_prim_step_tc (P : prog Λ) (e e': expr Λ) σ σ' K : 
+    prim_step_tc P e σ e' σ' → prim_step_tc P (fill K e) σ (fill K e') σ'. 
+  Proof. 
+    induction 1 as [ | e1 e2 e3 σ1 σ2 σ3 H1 H2 IH]; first (constructor; by apply fill_prim_step).
+    econstructor; last apply IH. by apply fill_prim_step.
+  Qed.
+   
+
+  Definition reach_stuck (P : prog Λ) (e : expr Λ) (σ : state Λ) :=
+    ∃ e' σ', prim_step_rtc P e σ e' σ' ∧ stuck P e' σ'.
+
+
+  (* TODO: move *)
+  Lemma prim_step_inv (P : prog Λ) e σ e' σ': prim_step P e σ e' σ' 
+    → ∃ K_redex e1 e2, e = fill K_redex e1 ∧ e' = fill K_redex e2 ∧ head_step P e1 σ e2 σ'. 
+  Proof. inversion 1. eauto 10. Qed.
+
+  (* TODO: move *)
+  Lemma fill_stuck (P : prog Λ) e σ K: stuck P e σ → stuck P (fill K e) σ.
+  Proof. 
+    intros Hstuck; split.
+    + apply fill_not_val, Hstuck.
+    + intros e'' σ'' (K_redex &e1 &e2 &Heq &-> &Hhead)%prim_step_inv.
+      edestruct (step_by_val P K K_redex _ _ _ _ _ Heq ltac:(apply Hstuck) Hhead) as (K'' & ->).
+      rewrite -fill_comp in Heq. apply fill_inj in Heq as ->.
+      eapply (proj2 Hstuck). econstructor; eauto.
+  Qed.
+
+  Lemma val_prim_step_rtc P v σ e' σ' : 
+    prim_step_rtc P (of_val v) σ e' σ' → e' = of_val v ∧ σ' = σ.
+  Proof. 
+    inversion 1; subst; first done. 
+    inversion H0; subst. 
+    edestruct (fill_val K e1') as (v1''& ?). 
+    { rewrite -H2. rewrite to_of_val. by exists v. } 
+    exfalso; eapply val_head_step.
+    erewrite <-(of_to_val e1') in H4; eauto.
+  Qed.
+
+  Lemma val_not_reach_stuck P v σ : ¬ reach_stuck P (of_val v) σ.
+  Proof. 
+    intros (e'&σ'& H & Hstuck). apply val_prim_step_rtc in H as (->&->).
+    destruct Hstuck as [H _]. rewrite to_of_val in H; discriminate.
+  Qed.
+
+  Lemma fill_reach_stuck (P : prog Λ) (e : expr Λ) K (σ : state Λ) :
+    reach_stuck P e σ → reach_stuck P (fill K e) σ.
+  Proof. 
+    intros (e' & σ' & [Hreach Hstuck]). exists (fill K e'), σ'. split.
+    - by apply fill_prim_step_rtc. 
+    - by apply fill_stuck.
+  Qed.
+
+  Lemma fill_reducible_prim_step P e e' σ σ' K: 
+    reducible P e σ → prim_step P (fill K e) σ e' σ' → ∃ e'', e' = fill K e'' ∧ prim_step P e σ e'' σ'.
+  Proof. 
+    (* TODO *)
+  Admitted. 
+
+End basic.
+
 
 Class simul_lang (PROP : bi) (Λ : language) := {
   (* state interpretation *)
@@ -29,10 +118,15 @@ Hint Mode simul_lang + - : typeclass_instances.
    greatest+least fp (stuttering) or just greatest fp (no stuttering). *)
 (* TODO: remove this TC once we don't need the no-stutter version anymore*)
 Class Sim {PROP : bi} {Λ : language} (s : simul_lang PROP Λ) := sim : expr Λ → expr Λ → (val Λ → val Λ → PROP) → PROP.
-Hint Mode Sim + + - : typeclass_instances.
+Hint Mode Sim - - - : typeclass_instances.
+
+(* FIXME: the notation with binders somehow does not work *) 
+Notation "et '⪯' es {{ v_t v_s , P }}" := (sim et es (λ v_t v_s, P)) (at level 40, v_t pattern, v_s pattern) : bi_scope.
+Notation "et '⪯' es {{ Φ }}" := (sim et es Φ) (at level 40) : bi_scope.
 
 (* discrete OFE instance for expr *)
 Definition exprO {Λ : language} := leibnizO (expr Λ).
+Instance expr_equiv {Λ} : Equiv (expr Λ). apply exprO. Defined.
 
 Section fix_lang.
   Context {PROP : bi}.
@@ -40,12 +134,11 @@ Section fix_lang.
   Context {Λ : language}.
   Context {s : simul_lang PROP Λ}.
 
-  Definition sim_expr {sim : Sim s} e_t e_s Φ := sim e_t e_s Φ.
   Definition sim_ectx {sim : Sim s} K_t K_s Φ :=
-    (∀ v_t v_s, val_rel v_t v_s -∗ sim_expr (fill K_t (of_val v_t)) (fill K_s (of_val v_s)) Φ)%I.
+    (∀ v_t v_s, val_rel v_t v_s -∗ sim (fill K_t (of_val v_t)) (fill K_s (of_val v_s)) Φ)%I.
 
   Implicit Types
-    (e_s e_t e: expr Λ)
+    (e_s e_t e: exprO (Λ := Λ))
     (P_s P_t P: prog Λ)
     (σ_s σ_t σ : state Λ).
 
@@ -56,10 +149,11 @@ Section fix_lang.
   Section stuttering.
     (** Simulation relation with stuttering *)
 
-    Definition least_step (Φ : val Λ → val Λ → PROP) (greatest_rec : expr Λ → expr Λ → PROP) (e_s : exprO) (least_rec : exprO → PROP) (e_t : exprO) :=
+    Definition least_step (Φ : val Λ → val Λ → PROP) (greatest_rec : exprO → exprO → PROP) (e_s : exprO) (least_rec : exprO → PROP) (e_t : exprO) :=
       (∀ P_t σ_t P_s σ_s, state_interp P_t σ_t P_s σ_s ∗ ¬ ⌜reach_stuck P_s e_s σ_s⌝ -∗ |==>
         (* value case *)
-        (∃ v_t v_s σ_s', ⌜to_val e_t = Some v_t⌝ ∗ ⌜prim_step_rtc P_s e_s σ_s (of_val v_s) σ_s'⌝ ∗ Φ v_t v_s)
+        (∃ v_t v_s σ_s', ⌜to_val e_t = Some v_t⌝ ∗ ⌜prim_step_rtc P_s e_s σ_s (of_val v_s) σ_s'⌝ ∗ 
+          state_interp P_t σ_t P_s σ_s' ∗ Φ v_t v_s)
 
         ∨ (* step case *)
         (⌜reducible P_t e_t σ_t⌝ ∗ ∀ e_t' σ_t', ⌜prim_step P_t e_t σ_t e_t' σ_t'⌝ -∗ |==>
@@ -155,17 +249,18 @@ Section fix_lang.
     Instance sim_stutter : Sim s. exact ((sim_aux).(unseal)). Defined.
     Definition sim_eq : sim_stutter = λ e_t e_s Φ, @sim_def Φ (e_s, e_t). by rewrite <- (sim_aux).(seal_eq). Defined.
 
-    Lemma sim_expr_unfold Φ e_t e_s:
-      sim_expr (sim:=sim_stutter) e_t e_s Φ ⊣⊢
+    Lemma sim_unfold Φ e_t e_s:
+      sim (Sim:=sim_stutter) e_t e_s Φ ⊣⊢
       (∀ P_t σ_t P_s σ_s, state_interp P_t σ_t P_s σ_s ∗ ¬ ⌜reach_stuck P_s e_s σ_s⌝ -∗ |==>
         (* value case *)
-          (∃ v_t v_s σ_s', ⌜to_val e_t = Some v_t⌝ ∗ ⌜prim_step_rtc P_s e_s σ_s (of_val v_s) σ_s'⌝ ∗ Φ v_t v_s)
+          (∃ v_t v_s σ_s', ⌜to_val e_t = Some v_t⌝ ∗ ⌜prim_step_rtc P_s e_s σ_s (of_val v_s) σ_s'⌝ ∗ 
+            state_interp P_t σ_t P_s σ_s' ∗ Φ v_t v_s)
 
         ∨ (* step case *)
         (⌜reducible P_t e_t σ_t⌝ ∗ ∀ e_t' σ_t', ⌜prim_step P_t e_t σ_t e_t' σ_t'⌝ -∗ |==>
-          (state_interp P_t σ_t' P_s σ_s ∗ sim_expr (sim:=sim_stutter) e_t' e_s Φ) ∨
+          (state_interp P_t σ_t' P_s σ_s ∗ sim (Sim:=sim_stutter) e_t' e_s Φ) ∨
           (∃ e_s' σ_s', ⌜prim_step_tc P_s e_s σ_s e_s' σ_s'⌝ ∗ state_interp P_t σ_t' P_s σ_s' ∗
-          sim_expr (sim:=sim_stutter) e_t' e_s' Φ))
+          sim (Sim:=sim_stutter) e_t' e_s' Φ))
 
         ∨ (* call case *)
         (∃ f K_t v_t K_s v_s σ_s', ⌜e_t = fill K_t (of_call f v_t)⌝ ∗
@@ -174,10 +269,229 @@ Section fix_lang.
           sim_ectx (sim:=sim_stutter) K_t K_s Φ)
       )%I.
     Proof.
-      rewrite /sim_ectx /sim_expr !sim_eq /uncurry sim_def_unfold /greatest_step.
+      rewrite /sim_ectx /sim !sim_eq /uncurry sim_def_unfold /greatest_step.
       rewrite least_def_unfold /least_step.
       by setoid_rewrite <-sim_def_least_def_unfold.
     Qed.
+
+    (* any post-fixed point is included in the gfp *)
+    Lemma sim_coind Φ (Ψ : exprO → exprO → PROP): 
+      Proper ((≡) ==> (≡) ==> (≡)) Ψ → 
+      ⊢ (□ ∀ e_t e_s, Ψ e_t e_s -∗ greatest_step Φ (λ '(e_s, e_t), Ψ e_t e_s) (e_s, e_t))
+        -∗ ∀ e_t e_s, Ψ e_t e_s -∗ sim e_t e_s Φ.
+    Proof. 
+      iIntros (Hp) "#H". iIntros (e_t e_s) "H0".
+      rewrite /sim sim_eq /sim_def.
+
+      set (Ψ_curry := (λ '(e_t, e_s), Ψ e_s e_t)).
+      assert (NonExpansive Ψ_curry) as Hne.
+      { intros ? [e1 e2] [e1' e2'] [H1 H2]. rewrite /Ψ_curry. cbn in H1, H2. 
+        apply equiv_dist, Hp. now apply discrete_iff in H1. now apply discrete_iff in H2. 
+      }
+      iApply (greatest_fixpoint_coind (greatest_step Φ) Ψ_curry).
+      { iModIntro. iIntros ([e_s' e_t']). iApply "H". } 
+      iApply "H0".
+    Qed.
+
+
+    (* TODO: not sure yet if this lemma is useful. if not, remove *)
+    Lemma sim_strong_ind' (e_s : exprO) Φ (Ψ : exprO → exprO → (val Λ → val Λ → PROP) → PROP): 
+      Proper ((≡) ==> (≡) ==> (pointwise_relation (val Λ) (pointwise_relation (val Λ) (≡))) ==> (≡)) Ψ → 
+      ⊢ (□ ∀ e_t, least_step Φ (uncurry (sim_def Φ)) e_s 
+              (λ e_t', Ψ e_t' e_s Φ ∧ least_def Φ (uncurry (sim_def Φ)) e_s e_t') 
+            e_t -∗ Ψ e_t e_s Φ)
+        -∗ ∀ e_t : exprO, (e_t ⪯ e_s {{ Φ }}) -∗ Ψ e_t e_s Φ.
+    Proof. 
+      iIntros (Hp) "#IH". iIntros (e_t).
+      rewrite /sim sim_eq /sim_def.
+      rewrite greatest_fixpoint_unfold {2}/greatest_step /least_def.
+
+      change (bi_greatest_fixpoint (greatest_step Φ)) with (sim_def Φ).
+      set (g_rec := least_step Φ (uncurry (sim_def Φ)) e_s). 
+
+      set (Ψ' := (λ e_t, Ψ e_t e_s Φ) : exprO → PROP).
+      iAssert ((□ (∀ e_t : exprO, g_rec (λ e_t' : exprO, Ψ' e_t' ∧ bi_least_fixpoint g_rec e_t') e_t -∗ Ψ' e_t)))%I as "#H".
+      { iModIntro. iApply "IH". } 
+      iPoseProof (least_fixpoint_strong_ind g_rec Ψ' with "H") as "Htemp".
+      unfold Ψ'. iApply "Htemp".
+    Qed.
+
+    (* TODO: not sure yet if this lemma is useful. if not, remove *)
+    Lemma sim_ind' (e_s : exprO) Φ (Ψ : exprO → exprO → (val Λ → val Λ → PROP) → PROP): 
+      Proper ((≡) ==> (≡) ==> (pointwise_relation (val Λ) (pointwise_relation (val Λ) (≡))) ==> (≡)) Ψ → 
+      ⊢ (□ ∀ e_t, least_step Φ (uncurry (sim_def Φ)) e_s (λ e_t', Ψ e_t' e_s Φ) e_t -∗ Ψ e_t e_s Φ)
+        -∗ ∀ e_t : exprO, e_t ⪯ e_s {{Φ}} -∗ Ψ e_t e_s Φ.
+    Proof. 
+      iIntros (Hp) "#IH". iApply sim_strong_ind'. iModIntro. 
+      iIntros (e_t) "H". iApply "IH".
+      iApply least_step_mon. 3: iApply "H". 2: auto.
+      iModIntro. by iIntros (e) "[H _]".
+    Qed.
+
+    Lemma sim_strong_ind greatest_rec (e_s : exprO) Φ (Ψ : exprO → PROP): 
+      Proper ((≡) ==> (≡)) Ψ → 
+      ⊢ (□ ∀ e_t, least_step Φ greatest_rec e_s 
+            (λ e_t', Ψ e_t' ∧ least_def Φ greatest_rec e_s e_t') 
+          e_t -∗ Ψ e_t)
+        -∗ ∀ e_t : exprO, least_def Φ greatest_rec e_s e_t -∗ Ψ e_t.
+    Proof. 
+      iIntros (Hp) "#H". iApply least_fixpoint_strong_ind.
+      iModIntro. iIntros (e_t) "IH". by iApply "H".
+    Qed.
+
+    Lemma sim_ind greatest_rec (e_s : exprO) Φ (Ψ : exprO → PROP): 
+      Proper ((≡) ==> (≡)) Ψ → 
+      ⊢ (□ ∀ e_t, least_step Φ greatest_rec e_s Ψ e_t -∗ Ψ e_t)
+        -∗ ∀ e_t : exprO, least_def Φ greatest_rec e_s e_t -∗ Ψ e_t.
+    Proof. iIntros (Hp) "#H". iApply least_fixpoint_ind. iModIntro. iIntros (e_t) "IH". by iApply "H". Qed.
+
+    Instance sim_proper : 
+      Proper (eq ==> eq ==> (pointwise_relation (val Λ) (pointwise_relation (val Λ) (≡))) ==> (≡)) sim.
+    Proof. 
+      intros e e' -> e1 e1' -> p1 p2 Heq2. 
+      rewrite /sim !sim_eq. apply greatest_fixpoint_proper; last reflexivity. 
+      intros p3 [e3 e3']. rewrite /greatest_step /least_def.
+      apply least_fixpoint_proper; last reflexivity. solve_proper.
+    Qed.
+
+    Lemma sim_value Φ v_t v_s: 
+      ⊢ Φ v_t v_s -∗ (of_val v_t) ⪯ (of_val v_s) {{Φ}}.
+    Proof. 
+      iIntros "Hv". rewrite sim_unfold. iIntros (????) "[Hstate Hreach]". 
+      iModIntro. iLeft. iExists (v_t), (v_s), (σ_s). iFrame. 
+      iSplitL. by rewrite to_of_val. eauto.
+    Qed.
+
+    Lemma bupd_sim Φ e_t e_s:
+      ⊢ (|==> e_t ⪯ e_s {{Φ}}) -∗ e_t ⪯ e_s {{Φ}}.
+    Proof. 
+      iIntros "Hv". rewrite sim_unfold. iIntros (????) "H". iMod "Hv". iApply ("Hv" with "H").
+    Qed.
+
+    Lemma sim_mono Φ Φ':
+      ⊢ (□ ∀ v_t v_s, Φ v_t v_s -∗ Φ' v_t v_s) 
+        → ∀ e_s e_t : exprO, e_t ⪯ e_s {{Φ}} -∗ e_t ⪯ e_s {{Φ'}}.
+    Proof.
+      iIntros "#Hmon". 
+      iIntros (e_s e_t) "H".
+      iApply (sim_coind Φ' (λ e_t e_s, e_t ⪯ e_s {{Φ}})%I); last done.
+      iModIntro. clear e_t e_s. iIntros (e_t e_s) "H".
+      rewrite /sim sim_eq sim_def_unfold. 
+      rewrite /greatest_step !least_def_unfold /least_step.
+      iIntros (????) "Hs". iSpecialize ("H" with "Hs"). iMod "H". iModIntro. 
+      iDestruct "H" as "[Hval | [Hred | Hcall]]". 
+      - iLeft. iDestruct "Hval" as (v_t v_s σ_s') "(?&?&?&?)". iExists v_t, v_s, σ_s'. iFrame. by iApply "Hmon".
+      - iRight; iLeft. iDestruct "Hred" as "[Hred Hstep]". iFrame. 
+        iIntros (e_t' σ_t') "Hprim". iMod ("Hstep" with "Hprim") as "[Hstutter | Hstep]"; iModIntro.
+        + iLeft. iDestruct "Hstutter" as "[Hstate Hleast]". iFrame.
+          (* inner induction *)
+          iApply sim_ind. 2: iApply "Hleast". clear P_t P_s σ_s σ_t σ_t' e_t.
+          iModIntro. iIntros (e_t) "IH". rewrite least_def_unfold /least_step. 
+          iIntros (P_t σ_t P_s σ_s) "H". iMod ("IH" with "H") as "IH". iModIntro.
+          iDestruct "IH" as "[Hval | [Hstep | Hcall]]". 
+          * iLeft. iDestruct "Hval" as (v_t v_s σ_s') "(?&?&?&?)". iExists v_t, v_s, σ_s'. iFrame. by iApply "Hmon".
+          * iRight; iLeft. iFrame.
+          * iRight; iRight. iFrame.
+        + iRight. iFrame.
+      - iRight; iRight. iFrame.
+    Qed.
+
+    Lemma sim_bind e_t e_s K_t K_s Φ: 
+      ⊢ e_t ⪯ e_s {{λ v_t v_s : val Λ, (∀ P_s σ_s, ¬ ⌜reach_stuck P_s (fill K_s (of_val v_s)) σ_s⌝) ∗
+          fill K_t (of_val v_t) ⪯ fill K_s (of_val v_s) {{Φ}} }}
+        -∗ fill K_t e_t ⪯ fill K_s e_s {{Φ}}.
+    Proof. 
+      iIntros "H".
+      iApply (sim_coind Φ (λ e_t' e_s', 
+        ∃ e_t e_s K_t K_s, ⌜e_t' = fill K_t e_t⌝ ∧ ⌜e_s' = fill K_s e_s⌝ ∧
+        e_t ⪯ e_s {{λ v_t v_s : val Λ, (∀ P_s σ_s, ¬ ⌜reach_stuck P_s (fill K_s (of_val v_s)) σ_s⌝) ∗ 
+            fill K_t (of_val v_t) ⪯ fill K_s (of_val v_s) {{Φ}}}})%I).
+      2: { iExists e_t, e_s, K_t, K_s. iFrame. eauto. } 
+      iModIntro. clear e_t e_s K_t K_s.
+      iIntros (e_t' e_s') "IH".
+      iDestruct "IH" as (e_t e_s K_t K_s) "[-> [-> H]]".
+      rewrite {1}/sim {1}sim_eq {1}sim_def_unfold. 
+      rewrite /greatest_step !least_def_unfold /least_step.
+
+      iIntros (????) "[Hs Hnreach]".
+      iMod ("H" with "[Hs Hnreach]") as "H". 
+      { iFrame. iIntros "%". iApply ("Hnreach" with "[%]"). by apply fill_reach_stuck. }
+      iDestruct "H" as "[Hval | [Hstep | Hcall]]". 
+      - iDestruct "Hval" as (v_t v_s σ_s') "(%& %&Hstate&[Hnreach Hpost])". 
+
+        (* unfold Hpost to examine the result and combine the two simulation proofs *)
+        rewrite {1}/sim {1}sim_eq {1}sim_def_unfold. 
+        rewrite {1}/greatest_step !least_def_unfold /least_step.
+        iMod ("Hpost" with "[Hstate Hnreach]") as "Hpost".   
+        { iFrame. iApply "Hnreach". } 
+        iModIntro.
+        iDestruct "Hpost" as "[Hv | [Hstep | Hcall]]". 
+        + iLeft. iDestruct "Hv" as (v_t' v_s' σ_s'') "(% & % & Hstate & Hpost)". 
+          iExists v_t', v_s', σ_s''. iFrame.
+          iSplitL. { iPureIntro. by rewrite -H1 (of_to_val _ _ H). } 
+          iPureIntro. 
+          eapply prim_step_rtc_trans. { apply fill_prim_step_rtc, H0. } 
+          assumption.
+        + iRight; iLeft. iDestruct "Hstep" as "[% Hstep]". iSplitR "Hstep".
+          { iPureIntro. by rewrite (of_to_val _ _ H) in H1. } 
+          iIntros (e_t' σ_t') "%". iMod ("Hstep" with "[]") as "Hstep". 
+          { iPureIntro. by rewrite (of_to_val _ _ H). } 
+          iModIntro. iDestruct "Hstep" as "[[Hstate Hstutter] | Hstep]".
+          * (* CA on the reduction of e_s to v_s to check if we need to stutter or not *)
+            apply (prim_step_rtc_tc_or) in H0 as [[-> ->] | H3].
+            { iLeft. iFrame. (* TODO *)
+              admit.
+            } 
+            iRight. iExists (fill K_s (of_val v_s)), σ_s'. iFrame.
+            iSplitR "Hstutter". 
+            { iPureIntro. by apply fill_prim_step_tc. }
+            cbn. iExists e_t', (of_val v_s), empty_ectx, K_s. rewrite fill_empty.
+            do 2 (iSplitL ""; first auto).
+            (* TODO *)
+            admit.
+          * iDestruct "Hstep" as (e_s' σ_s'') "(%&Hstate& Hrec)". iRight. 
+            iExists e_s', σ_s''. iFrame. iSplitL "".
+            { iPureIntro. eapply prim_step_rtc_tc_trans; last eassumption. by apply fill_prim_step_rtc. } 
+            cbn. iExists e_t', e_s', empty_ectx, empty_ectx. rewrite !fill_empty. 
+            do 2 (iSplitL ""; first auto). 
+            iApply sim_mono. 2: { rewrite /sim sim_eq. iApply "Hrec". }
+            iModIntro. iIntros (??) "H". rewrite !fill_empty. iSplitL "". 
+            { iIntros (??) "%". iPureIntro. by eapply val_not_reach_stuck. } 
+            by iApply sim_value.
+        + iDestruct "Hcall" as (f K_t' v_t' K_s' v_s' σ_s'') "Hcall". iRight; iRight.
+          admit. (* TODO *)
+      - (* simply thread through everything *)
+        iModIntro. iRight; iLeft. iDestruct "Hstep" as "[% Hstep]".
+        iSplitL "". { iPureIntro. by apply fill_reducible. }
+        iIntros (e_t' σ_t') "%". 
+        destruct (fill_reducible_prim_step _ _ _ _ _ _ H H0) as (e_t'' & -> & H1). 
+        iMod ("Hstep" with "[]") as "Hstep". { iPureIntro. apply H1. }
+        iModIntro. iDestruct "Hstep" as "[[Hstate Hstutter] | Hstep]". 
+        + iLeft. iFrame.
+          (* TODO : inner induction *)
+          admit.
+        + iRight. iDestruct "Hstep" as (e_s' σ_s') "(% & Hstate & Hrec)". 
+          iExists (fill K_s e_s'), σ_s'. iFrame. iSplitL "". 
+          { iPureIntro. by apply fill_prim_step_tc. }
+          cbn. iExists e_t'', e_s', K_t, K_s. 
+          do 2 (iSplitL ""; first auto). 
+          rewrite /sim sim_eq. iApply "Hrec".
+      - (* simply thread through everything *)
+        iModIntro. iRight; iRight. 
+        iDestruct "Hcall" as (f K_t' v_t K_s' v_s σ_s') "(-> & % & Hval & Hstate & Hrec)".
+        iExists f, (comp_ectx K_t K_t'), v_t, (comp_ectx K_s K_s'), v_s, σ_s'. 
+        iSplitL "". by rewrite fill_comp. 
+        iSplitL "". { iPureIntro. rewrite -fill_comp. by apply fill_prim_step_rtc. } 
+        iFrame. 
+        iIntros (v_t' v_s') "Hv". iSpecialize ("Hrec" with "Hv"). cbn. 
+        iExists (fill K_t' (of_val v_t')), (fill K_s' (of_val v_s')), K_t, K_s. 
+        iSplitL "". by rewrite -fill_comp. iSplitL "". by rewrite -fill_comp. 
+        rewrite /sim sim_eq. iApply "Hrec".
+    Admitted.
+
+    
+    (** Corollaries *)
+
 
   End stuttering.
 
@@ -187,7 +501,8 @@ Section fix_lang.
     Definition step_nostutter (Φ : val Λ → val Λ → PROP) (greatest_rec : exprO * exprO → PROP) : exprO * exprO → PROP:=
       λ '(e_s, e_t), (∀ P_t σ_t P_s σ_s, state_interp P_t σ_t P_s σ_s ∗ ¬ ⌜reach_stuck P_s e_s σ_s⌝ -∗ |==>
         (* value case *)
-        (∃ v_t v_s σ_s', ⌜to_val e_t = Some v_t⌝ ∗ ⌜prim_step_rtc P_s e_s σ_s (of_val v_s) σ_s'⌝ ∗ Φ v_t v_s)
+        (∃ v_t v_s σ_s', ⌜to_val e_t = Some v_t⌝ ∗ ⌜prim_step_rtc P_s e_s σ_s (of_val v_s) σ_s'⌝ ∗ 
+          state_interp P_t σ_t P_s σ_s' ∗ Φ v_t v_s)
 
         ∨ (* step case *)
         (⌜reducible P_t e_t σ_t⌝ ∗ ∀ e_t' σ_t', ⌜prim_step P_t e_t σ_t e_t' σ_t'⌝ -∗ |==>
@@ -203,8 +518,10 @@ Section fix_lang.
     Definition sim_nostutter_def (Φ : val Λ → val Λ → PROP) :=
       bi_greatest_fixpoint (step_nostutter Φ).
 
-    Instance step_nostutter_proper Φ rec:
-      Proper ((≡) ==> (≡)) (step_nostutter Φ rec).
+    Instance step_nostutter_proper:
+      Proper ((pointwise_relation (val Λ) (pointwise_relation (val Λ) (≡))) 
+        ==> (pointwise_relation _ (≡)) 
+        ==> (≡) ==> (≡)) (step_nostutter).
     Proof. solve_proper. Qed.
 
     Instance step_nostutter_mono (Φ : val Λ → val Λ → PROP):
@@ -236,16 +553,17 @@ Section fix_lang.
     Definition sim_nostutter_eq : sim_nostutter = λ e_t e_s Φ, @sim_nostutter_def Φ (e_s, e_t).
       by rewrite <- (sim_nostutter_aux).(seal_eq). Defined.
 
-    Lemma sim_expr_unfold_nostutter e_t e_s Φ:
-      sim_expr (sim:=sim_nostutter) e_t e_s Φ ⊣⊢
+    Lemma sim_nostutter_unfold e_t e_s Φ:
+      sim (Sim:=sim_nostutter) e_t e_s Φ ⊣⊢
       (∀ P_t σ_t P_s σ_s, state_interp P_t σ_t P_s σ_s ∗ ¬ ⌜reach_stuck P_s e_s σ_s⌝ -∗ |==>
         (* value case *)
-          (∃ v_t v_s σ_s', ⌜to_val e_t = Some v_t⌝ ∗ ⌜prim_step_rtc P_s e_s σ_s (of_val v_s) σ_s'⌝ ∗ Φ v_t v_s)
+          (∃ v_t v_s σ_s', ⌜to_val e_t = Some v_t⌝ ∗ ⌜prim_step_rtc P_s e_s σ_s (of_val v_s) σ_s'⌝ ∗ 
+            state_interp P_t σ_t P_s σ_s' ∗ Φ v_t v_s)
 
         ∨ (* step case *)
         (⌜reducible P_t e_t σ_t⌝ ∗ ∀ e_t' σ_t', ⌜prim_step P_t e_t σ_t e_t' σ_t'⌝ -∗ |==>
           ∃ e_s' σ_s', ⌜prim_step_tc P_s e_s σ_s e_s' σ_s'⌝ ∗ state_interp P_t σ_t' P_s σ_s' ∗
-          sim_expr (sim:=sim_nostutter) e_t' e_s' Φ)
+          sim (Sim:=sim_nostutter) e_t' e_s' Φ)
 
         ∨ (* call case *)
         (∃ f K_t v_t K_s v_s σ_s', ⌜e_t = fill K_t (of_call f v_t)⌝ ∗
@@ -254,7 +572,49 @@ Section fix_lang.
           sim_ectx (sim:=sim_nostutter) K_t K_s Φ)
       )%I.
     Proof.
-      by rewrite /sim_ectx /sim_expr !sim_nostutter_eq /uncurry sim_nostutter_def_unfold /step_nostutter.
+      by rewrite /sim_ectx /sim !sim_nostutter_eq /uncurry sim_nostutter_def_unfold /step_nostutter.
     Qed.
+
+    Lemma sim_nostutter_coind (Ψ : exprO → exprO → (val Λ → val Λ → PROP) → PROP): 
+      Proper ((≡) ==> (≡) ==> (pointwise_relation (val Λ) (pointwise_relation (val Λ) (≡))) ==> (≡)) Ψ → 
+      ⊢ (□ ∀ e_t e_s Φ, Ψ e_t e_s Φ -∗ step_nostutter Φ (λ '(e_s', e_t'), Ψ e_t' e_s' Φ) (e_s, e_t))
+        → (∀ e_t e_s Φ, Ψ e_t e_s Φ -∗ e_t ⪯ e_s {{Φ}}).
+    Proof. 
+      iIntros (Hp) "#IH". iIntros (e_t e_s Φ) "H".
+      rewrite /sim sim_nostutter_eq /sim_nostutter_def.
+      set (Ψ_curry := (λ '(e_t, e_s), Ψ e_s e_t Φ)).
+      assert (NonExpansive Ψ_curry) as Hne.
+      { intros ? [e1 e2] [e1' e2'] [H1 H2]. rewrite /Ψ_curry. cbn in H1, H2. 
+        apply equiv_dist, Hp. now apply discrete_iff in H1. now apply discrete_iff in H2. 
+        reflexivity. 
+      }
+
+      iApply (greatest_fixpoint_coind (step_nostutter Φ) Ψ_curry with "[]").
+      { iModIntro. iIntros ([e_s' e_t']) "H'". by iApply "IH". }
+      iApply "H".
+    Qed.
+
+    Instance sim_nostutter_proper : 
+      Proper (eq ==> eq ==> (pointwise_relation (val Λ) (pointwise_relation (val Λ) (≡))) ==> (≡)) sim.
+    Proof. 
+      intros e e' -> e1 e1' -> p1 p2 Heq2. 
+      rewrite /sim !sim_nostutter_eq. apply greatest_fixpoint_proper; solve_proper.
+    Qed.
+
+    Lemma sim_nostutter_value Φ v_t v_s: 
+      ⊢ Φ v_t v_s -∗ (of_val v_t) ⪯ (of_val v_s) {{Φ}}.
+    Proof. 
+      iIntros "Hv". rewrite sim_nostutter_unfold. iIntros (????) "[Hstate Hreach]". 
+      iModIntro. iLeft. iExists (v_t), (v_s), (σ_s). iFrame. 
+      iSplitL. by rewrite to_of_val. eauto.
+    Qed.
+
+    Lemma bupd_sim_nostutter Φ e_t e_s:
+      ⊢ (|==> e_t ⪯ e_s {{Φ}}) -∗ e_t ⪯ e_s {{Φ}}.
+    Proof. 
+      iIntros "Hv". rewrite sim_nostutter_unfold. iIntros (????) "H". iMod "Hv". iApply ("Hv" with "H").
+    Qed.
+
   End no_stuttering.
 End fix_lang.
+
